rsp.fst
@@ -8,112 +8,365 @@ open IOStHist
 open M4
 open Minterop
 
-type set_of_traces = events_trace -> Type0
+type set_of_traces (a:Type) = events_trace * a -> Type0
 
-val included_in : set_of_traces -> set_of_traces -> Type0
-let included_in s1 s2 = forall t. s1 t ==>  s2 t
+val included_in : (#a:Type) -> (#b:Type) -> (b -> a) -> set_of_traces a -> set_of_traces b -> Type0
+let included_in rel s1 s2 = forall t r1. s1 (t, r1) ==>  (exists r2. rel r2 == r1 /\ s2 (t, r2))
 
 let rec behavior #a
-  (m : io a) : set_of_traces =
+  (m : io a) : set_of_traces (maybe a) =
   match m with
-  | Return x -> fun t -> t == []
-  | Throw err -> fun t -> t == []
+  | Return x -> fun t -> t == ([], Inl x)
+  | Throw err -> fun t -> t == ([], Inr err)
   | Cont t -> begin
     match t with
-    | Call cmd args fnc -> (fun t' -> 
-      (exists res t. (
+    | Call cmd args fnc -> (fun (t', r') -> 
+      (exists (res:resm cmd) t. (
          FStar.WellFounded.axiom1 fnc res;
-         (behavior (fnc res) t) /\
-         t' == ((convert_call_to_event cmd args res)::t))))
+         (behavior (fnc res) (t,r')) /\
+         t' == (convert_call_to_event cmd args res)::t)))
   end
 
-let empty_set : set_of_traces = fun t -> t == []
+let empty_set (#a:Type) () : set_of_traces a = fun (t,r) -> t == []
 
-let export_empty_set (a:Type) {| exportable a |} ()
-  : Lemma (forall (x:a). behavior (io_return _ (export x)) `included_in` empty_set) = ()
+let id #a (x:a) = x
 
-let ibind_f_export 
-  #t2 {| d:exportable t2 |}
-  (f:io t2) :
+let beh_shift_trace
+  #a
+  (cmd : io_cmds)
+  (argz : args cmd)
+  (rez : resm cmd)
+  (fnc : resm cmd -> io a)
+  (t:events_trace)
+  (r:maybe a) :
+  Lemma 
+    (requires (behavior (Cont (Call cmd argz fnc)) ((convert_call_to_event cmd argz rez :: t), r)))
+    (ensures (behavior (fnc rez) (t, r))) = 
+  () 
+
+let beh_extend_trace 
+  #a
+  (cmd : io_cmds)
+  (argz : args cmd)
+  (rez : resm cmd)
+  (fnc : resm cmd -> io a)
+  (t:events_trace)
+  (r:maybe a) :
   Lemma
-    (included_in
-      (behavior f)
-      (behavior (io_bind t2 d.etype f (fun x -> io_return _ (export x))))) 
-  by (
-    explode ();
-    dump "h"
-  ) = 
-  export_empty_set t2 ();
+    (requires (behavior (fnc rez) (t, r)))
+    (ensures (behavior (Cont (Call cmd argz fnc)) ((convert_call_to_event cmd argz rez) :: t, r))) 
+  by (compute ()) = 
   ()
 
+let beh_extend_trace_d
+  #a
+  (cmd : io_cmds)
+  (argz : args cmd)
+  (rez : resm cmd)
+  (fnc : resm cmd -> io a)
+  (t:events_trace) :
+  Lemma
+    (forall r. (behavior (fnc rez) (t, r) ==>
+      (behavior (Cont (Call cmd argz fnc)) ((convert_call_to_event cmd argz rez) :: t, r)))) =
+  Classical.forall_intro (
+    Classical.move_requires (beh_extend_trace cmd argz rez fnc t))
+
+let beh_extend_trace_in_bind 
+  #a #b
+  (cmd : io_cmds)
+  (argz : args cmd)
+  (rez : resm cmd)
+  (fnc : resm cmd -> io a)
+  (k : a -> io b)
+  (t:events_trace)
+  (r:maybe b) :
+  Lemma
+    (requires (behavior (io_bind a b (fnc rez) k) (t, r))) 
+    (ensures (behavior (io_bind a b (Cont (Call cmd argz fnc)) k) ((convert_call_to_event cmd argz rez) :: t, r))) =
+  calc (==) {
+    io_bind a b (Cont (Call cmd argz fnc)) k;
+    == {}
+    sys_bind io_cmds io_cmd_sig a b (Cont (Call cmd argz fnc)) k;
+    == { _ by (norm [iota; delta]; compute ()) }
+    Cont (sysf_fmap (fun fnci -> 
+      sys_bind io_cmds io_cmd_sig a b fnci k) (Call cmd argz fnc));
+    == { _ by (unfold_def(`sysf_fmap); norm [iota]; unfold_def(`io_bind)) }
+    Cont (Call cmd argz (fun rez -> 
+      io_bind a b (fnc rez) k));
+  };
+  beh_extend_trace cmd argz rez (fun rez -> io_bind a b (fnc rez) k) t r;
+  assert (behavior (Cont (Call cmd argz (fun rez -> 
+    io_bind a b (fnc rez) k))) ((convert_call_to_event cmd argz rez) :: t, r)) by (
+    unfold_def (`convert_call_to_event); assumption ())
+
+let extract_result (cmd:io_cmds) (event:io_event) : 
+  Pure (resm cmd)
+    (requires ((cmd == Openfile /\ EOpenfile? event) \/
+               (cmd == Read /\ ERead? event) \/
+               (cmd == Close /\ EClose? event)))
+    (ensures (fun r -> True)) = 
+  match cmd with 
+  | Openfile -> EOpenfile?.r event 
+  | Read -> ERead?.r event 
+  | Close -> EClose?.r event 
+    
+let rec beh_bind_inl
+  #a #b
+  (m : io a)
+  (k : a -> io b) 
+  (r1:a) 
+  (t1 t2 : events_trace)
+  (r2:maybe b) :
+  Lemma 
+    (requires (behavior m (t1, (Inl r1)) /\ behavior (k r1) (t2, r2)))
+    (ensures (behavior (io_bind _ _ m k) (t1 @ t2, r2))) =
+  match m with
+  | Return x -> ()
+  | Throw err -> ()
+  | Cont (Call cmd argz fnc) -> begin
+    let (ht1 :: tt1) = t1 in
+    let rez : resm cmd = extract_result cmd ht1 in
+    FStar.WellFounded.axiom1 fnc rez;
+    beh_shift_trace cmd argz rez fnc tt1 (Inl r1);
+    beh_bind_inl (fnc rez) k r1 tt1 t2 r2;
+    beh_extend_trace_in_bind cmd argz rez fnc k (tt1@t2) r2
+  end
+  
+let rec beh_bind_inr
+  #a #b
+  (m : io a)
+  (k : a -> io b)
+  (r1:exn)
+  (t1 : events_trace) :
+  Lemma 
+    (requires (behavior m (t1, (Inr r1))))
+    (ensures (behavior (io_bind _ _ m k) (t1, (Inr r1)))) =
+  match m with
+  | Throw err -> ()
+  | Cont (Call cmd argz fnc) -> begin
+    let (ht1 :: tt1) = t1 in
+    let rez : resm cmd = extract_result cmd ht1 in
+    FStar.WellFounded.axiom1 fnc rez;
+    beh_shift_trace cmd argz rez fnc tt1 (Inr r1);
+    beh_bind_inr (fnc rez) k r1 tt1;
+    beh_extend_trace_in_bind cmd argz rez fnc k (tt1) (Inr r1)
+  end
+
+let beh_bind_0 
+  #a #b
+  (m : io a)
+  (k : a -> io b) 
+  (r1:maybe a) :
+  Lemma (forall t1.
+    behavior m (t1, r1) ==>
+      (Inr? r1 ==>  behavior (io_bind _ _ m k) (t1, (Inr (Inr?.v r1)))) /\
+      (Inl? r1 ==>  (forall t2 r2. (behavior (k (Inl?.v r1)) (t2, r2) ==>  
+                     behavior (io_bind _ _ m k) (t1 @ t2, r2))))) =
+  if (Inr? r1) then (
+    Classical.forall_intro (
+      Classical.move_requires (beh_bind_inr m k (Inr?.v r1)))
+  ) else (
+    Classical.forall_intro_3 (
+      Classical.move_requires_3 (beh_bind_inl m k (Inl?.v r1)))
+  )
+
+let beh_bind
+  #a #b
+  (m : io a)
+  (k : a -> io b) :
+  Lemma (forall (r1:maybe a) t1.
+    behavior m (t1, r1) ==>
+      (Inr? r1 ==>  behavior (io_bind _ _ m k) (t1, (Inr (Inr?.v r1)))) /\
+      (Inl? r1 ==>  (forall t2 r2. behavior (k (Inl?.v r1)) (t2, r2) ==>  
+                              behavior (io_bind _ _ m k) (t1 @ t2, r2)))) =
+  Classical.forall_intro (beh_bind_0 m k)
+
+unfold let inl_app #a #b (f:a -> b) (x:maybe a) : maybe b =
+  match x with
+  | Inl x -> Inl (f x)
+  | Inr err -> Inr err
+
+let rec beh_bind_tot_0
+  #a #b
+  (f:io a) 
+  (g:a -> Tot b)
+  (r1:maybe b)
+  (t:events_trace) :
+  Lemma 
+    (requires (behavior (io_bind a b f (fun x -> lift_pure_m4wp b (fun p -> p (g x)) (fun _ -> g x) (fun _ -> True))) (t, r1)))
+    (ensures (exists r2. inl_app g r2 == r1 /\ behavior f (t, r2)))  =
+  match f with
+  | Return x -> 
+      assert (inl_app g (Inl x) == r1);
+      assert (behavior f (t, (Inl x)))
+  | Throw err -> 
+      assert (inl_app g (Inr err) == r1);
+      assert (behavior f (t, (Inr err)))
+  | Cont (Call cmd argz fnc) ->
+    let (ht1 :: tt1) = t in
+    let rez : resm cmd = extract_result cmd ht1 in
+    FStar.WellFounded.axiom1 fnc rez;
+    beh_bind_tot_0 (fnc rez) g r1 tt1;
+    beh_extend_trace_d cmd argz rez fnc (tt1)
+       
+let beh_bind_tot
+  #a #b
+  (f:io a)
+  (g:a -> Tot b) :
+  Lemma 
+    (forall r1 t. (behavior (io_bind a b f (fun x -> lift_pure_m4wp b (fun p -> p (g x)) (fun _ -> g x) (fun _ -> True))) (t, r1)) ==>  (exists r2. r1 == inl_app g r2 /\ behavior f (t,r2))) =
+  Classical.forall_intro_2 (Classical.move_requires_2 (beh_bind_tot_0 f g))
+
+let beh_included_bind_tot
+  #a #b
+  (f:io a) 
+  (g:a -> Tot b) :
+  Lemma
+    (included_in (inl_app g)
+      (behavior (io_bind a b f (fun x -> lift_pure_m4wp b (fun p -> p (g x)) (fun _ -> g x) (fun _ -> True))))
+      (behavior f)) = 
+  beh_bind_tot f g
+  
+let cdr #a (_, (x:a)) : a = x
 
 let iost_to_io #t2 (tree : io (events_trace * t2)) : io t2 =
-  match tree with
-  | Return (s1, r) -> Return r
-  | Throw r -> Throw r
-  | Cont (Call cmd argz fnc) ->
-    io_bind (events_trace * t2) t2
-      (Cont (Call cmd argz fnc))
-      (fun (_, r) -> io_return _ r)
+  io_bind (events_trace * t2) t2
+    tree
+    (fun r -> io_return _ (cdr r))
 
-let behavior_iost_to_io () : 
-  Lemma (forall (a:Type) (tree:io (events_trace * a)). 
-    behavior (iost_to_io tree) `included_in` behavior tree) = admit ()
-
-
+let beh_iost_to_io (a:Type) (tree:io (events_trace * a)) :
+  Lemma (behavior (iost_to_io tree) `included_in (inl_app cdr)` behavior tree) 
+  by (unfold_def (`iost_to_io); norm [iota;delta]; compute ()) =
+  beh_included_bind_tot #(events_trace * a) #a
+    tree
+    cdr
 
 unfold let ref #a (x : io a) : M4.irepr a (fun p -> forall res. p res) = (fun _ -> x)
 
-let _export_IOStHist_lemma #t1 #t2
-  {| d1:importable t1 |}
-  {| d2:exportable t2 |}
-  (pre : t1 -> events_trace -> Type0)
-  {| checkable2 pre |}
+let beh_included_in_trans_id x y z :
+  Lemma (
+    (behavior x `included_in id` behavior y /\
+    behavior y `included_in id` behavior z) ==>
+      behavior x `included_in id` behavior z) = ()
+  
+let beh_included_in_trans_id_g x y z g:
+  Lemma (
+    (behavior x `included_in id` behavior y /\
+    behavior y `included_in g` behavior z) ==>
+      behavior x `included_in g` behavior z) = ()
+  
+let beh_included_in_trans_g_id x y z g:
+  Lemma (
+    (behavior x `included_in g` behavior y /\
+    behavior y `included_in id` behavior z) ==>
+      behavior x `included_in g` behavior z) = ()
+
+let compose g f = fun x -> g (f x)
+
+let beh_included_in_merge_f_g x y z f g:
+  Lemma (
+    (behavior x `included_in f` behavior y /\
+    behavior y `included_in g` behavior z) ==>
+      behavior x `included_in (compose f g)` behavior z) = ()
+
+let _export_IOStHist_lemma
+  #t1 {| d1:importable t1 |} 
+  #t2 {| d2:exportable t2 |}
+  (pre : t1 -> events_trace -> Type0) {| checkable2 pre |}
   (post : t1 -> events_trace -> maybe (events_trace * t2) -> events_trace -> Type0)
   (f:(x:t1 -> IOStHist t2 (pre x) (post x))) 
   (x':d1.itype) : 
-  Lemma (match import x' with
+  Lemma (
+    let ef : d1.itype -> M4 d2.etype = _export_IOStHist_arrow_spec pre post f in
+    let res' = reify (ef x') (fun _ -> True) in
+    match import x' with
     | Some x -> (
-        let ef : d1.itype -> M4 d2.etype = _export_IOStHist_arrow_spec pre post f in
-        let res' = reify (ef x') (fun _ -> True) in
+      let f' = reify (f x) (post x []) in
+      (check2 #t1 #events_trace #pre x [] ==>  
+        behavior res' `included_in (inl_app (compose export cdr))` behavior (f' [])) /\
+      (~(check2 #t1 #events_trace #pre x []) ==>  
+        behavior res' `included_in id` empty_set ()))
+    | None -> behavior res' `included_in id` empty_set ()) =
 
-        let f' = reify (f x) (post x []) in
-        check2 #t1 #events_trace #pre x [] ==>  behavior res' `included_in` behavior (f' []))
-        // TODO: prove that behavior of res is empty trace if check2 fails?
-    | None -> 
-       // TODO: prove that behavior of res is the empty trace if import fails?
-           True)=
-
+  let ef : d1.itype -> M4 d2.etype = _export_IOStHist_arrow_spec pre post f in
+  let included_in_id #a = included_in #a #a (id #a) in
   match import x' with
   | Some x -> begin
     if (check2 #t1 #events_trace #pre x []) then (
-        let ef : d1.itype -> M4 d2.etype = _export_IOStHist_arrow_spec pre post f in
-        calc (included_in) {
+        calc (included_in_id) {
             behavior (reify (ef x') (fun _ -> True));
-            `included_in` {}
+            `included_in_id` {}
             behavior (reify ((_export_IOStHist_arrow_spec pre post f <: (d1.itype -> M4 d2.etype)) x') (fun _ -> True));
-            `included_in` { _ by (unfold_def(`_export_IOStHist_arrow_spec); norm [delta]) }
+            // TODO: Cezar: The idea behind this is to get rid of the `match` and the `if` 
+            // because we did them already in the proof.
+            `included_in_id` { _ by (unfold_def(`_export_IOStHist_arrow_spec); norm [delta]; tadmit (); dump "h") }
             behavior (reify (
               (export (M4wp?.reflect (ref (iost_to_io (reify (f x) (post x []) []))) <: M4wp t2 (fun p -> forall res. p res)) <: d2.etype)) (fun _ -> True));
-            == { admit () } // unfold reify
-            // Cezar: is the 3rd argument correct? I suppose it should pre and post
+            // TODO: Cezar: this should be just an unfolding of `reify`. I talked with Guido
+            // and it seems using tactics is not a solution to unfold `reify` for 
+            // layered effects because: "reification of layered effects is explicitly disabled
+            // since it requires producing the indices for the bind, and we do not store them
+            // anywhere". I tried to manually unfold looking at EMF* (Dijkstra Monads for
+            // Free), but it seems that F* does not accept this proof. I created a new file only
+            // for this problem: `UnfoldReify.fst`.
+            `included_in_id` { admit () }
+            // TODO: Cezar: is the 3rd argument correct? I suppose it should use pre and post
             behavior (M4.ibind t2 d2.etype (fun p -> forall res. p res) (fun x -> m4_return_wp (d2.etype) (export x))
                 (reify (M4wp?.reflect (ref (iost_to_io (reify (f x) (post x []) []))) <: M4wp t2 (fun p -> forall res. p res)))
                 (fun x -> lift_pure_m4wp d2.etype (fun p -> p (export x)) (fun _ -> export x)) (fun _ -> True));
-            `included_in` { _ by (unfold_def (`ibind); dump "H"); admit () }
-            behavior (M4.ibind t2 d2.etype (fun p -> forall res. p res) (fun x -> m4_return_wp (d2.etype) (export x))
-                (ref (iost_to_io (reify (f x) (post x []) [])))
-                (fun x -> lift_pure_m4wp d2.etype (fun p -> p (export x)) (fun _ -> export x)) (fun _ -> True));
-        //     `included_in` { test  (ref (iost_to_io (reify (f x) (post x []) []))) }
-        //     // `included_in` { _ by (norm [iota]; dump "h") }
+        };
+
+        beh_included_bind_tot #t2 #d2.etype
+          (reify (M4wp?.reflect (ref (iost_to_io (reify (f x) (post x []) []))) <: M4wp t2 (fun p -> forall res. p res)) (compute_post t2 (Mkexportable?.etype d2) (fun x -> m4_return_wp (Mkexportable?.etype d2) (export x)) (fun _ -> True)))
+            export;
+
+        assert (
+            (behavior (M4.ibind t2 d2.etype (fun p -> forall res. p res) (fun x -> m4_return_wp (d2.etype) (export x))
+                (reify (M4wp?.reflect (ref (iost_to_io (reify (f x) (post x []) []))) <: M4wp t2 (fun p -> forall res. p res)))
+                (fun x -> lift_pure_m4wp d2.etype (fun p -> p (export x)) (fun _ -> export x)) (fun _ -> True)))
+          `included_in (inl_app export)`
+            (behavior (reify (M4wp?.reflect (ref (iost_to_io (reify (f x) (post x []) []))) <: M4wp t2 (fun p -> forall res. p res)) (fun _ -> True)))
+        ) by (unfold_def (`ibind));
+
+       calc (included_in_id) {
+         behavior (reify (M4wp?.reflect (ref (iost_to_io (reify (f x) (post x []) []))) <: M4wp t2 (fun p -> forall res. p res)) (fun _ -> True));
+         `included_in_id` {}
+         behavior (iost_to_io (reify (f x) (post x []) []));
+       };
+
+       beh_iost_to_io t2 (reify (f x) (post x []) []);
+
+       assert (
+         behavior (iost_to_io (reify (f x) (post x []) []))
+         `included_in (inl_app cdr)` 
+         behavior (reify (f x) (post x []) []))
+    ) else begin
+        calc (==) {
+            reify (ef x') (fun _ -> True);
+            == {}
+            reify ((_export_IOStHist_arrow_spec pre post f <: (d1.itype -> M4 d2.etype)) x') (fun _ -> True);
+            == { 
+            _ by (unfold_def(`_export_IOStHist_arrow_spec); norm [iota]; tadmit (); dump "h") }
+            reify (M4.raise Contract_failure) (fun _ -> True);
+            // TODO: Cezar: The idea behind this is to get rid of the `match` and the `if` 
+            // because we did them already in the proof.
             == { admit () }
-            behavior (iost_to_io (reify (f x) (post x []) []));
-            `included_in` { behavior_iost_to_io () }
-            behavior (reify (f x) (post x []) []);
+            Throw Contract_failure;
         }
-    ) else ()
+    end
   end
-  | None -> ()
+  | None -> begin
+    calc (==) {
+        reify (ef x') (fun _ -> True);
+        == {}
+        reify ((_export_IOStHist_arrow_spec pre post f <: (d1.itype -> M4 d2.etype)) x') (fun _ -> True);
+        == { 
+          _ by (unfold_def(`_export_IOStHist_arrow_spec); norm [iota]; tadmit (); dump "h") }
+        reify (M4.raise Contract_failure) (fun _ -> True);
+        == { admit () }
+        Throw Contract_failure;
+    }
+  end
 
 
 let export_IOStHist_lemma 
@@ -123,17 +376,17 @@ let export_IOStHist_lemma
   (post : t1 -> events_trace -> maybe (events_trace * t2) -> events_trace -> Type0)
   (f:(x:t1 -> IOStHist t2 (pre x) (post x))) : 
   Lemma (forall (x':d1.itype). (
+    let ef : d1.itype -> M4 d2.etype = _export_IOStHist_arrow_spec pre post f in
+    let res' = reify (ef x') (fun _ -> True) in
     match import x' with
     | Some x -> (
-        let ef : d1.itype -> M4 d2.etype = export f in
-        let res' = reify (ef x') (fun _ -> True) in
-
-        let f' = reify (f x) (post x []) in
-
-        check2 #t1 #events_trace #pre x [] == true ==>  behavior res' `included_in` behavior (f' []))
-    | None -> True)) =
-  Classical.forall_intro (_export_IOStHist_lemma #t1 #t2 pre post f)
-
+      let f' = reify (f x) (post x []) in
+      (check2 #t1 #events_trace #pre x [] ==>  
+        behavior res' `included_in (inl_app (compose export cdr))` behavior (f' [])) /\
+      (~(check2 #t1 #events_trace #pre x []) ==>  
+        behavior res' `included_in id` empty_set ()))
+    | None -> behavior res' `included_in id` empty_set ())) =
+  Classical.forall_intro (_export_IOStHist_lemma #t1 #d1 #t2 #d2 pre post f)
 
 let export_GIO_lemma 
   #t1 {| d1:importable t1 |} 
@@ -141,61 +394,75 @@ let export_GIO_lemma
   (pi:check_type)
   (f:(x:t1 -> GIO t2 pi)) : 
   Lemma (forall (x':d1.itype). (
+    let ef : d1.itype -> M4 d2.etype = export f in
+    let res' = reify (ef x') (fun _ -> True) in
     match import x' with
     | Some x -> (
-        let ef : d1.itype -> M4 d2.etype = export f in
-        let res' = reify (ef x') (fun _ -> True) in
-
-        let f' = reify (f x) (gio_post pi []) in
-
-        check2 #t1 #events_trace #(fun _ -> gio_pre pi) x [] == true ==>  behavior res' `included_in` behavior (f' []))
-    | None -> True)) =
+      let f' = reify (f x) (gio_post pi []) in
+      (check2 #t1 #events_trace #(fun _ -> gio_pre pi) x [] ==>  
+        behavior res' `included_in (inl_app (compose export cdr))` behavior (f' [])) /\
+      (~(check2 #t1 #events_trace #(fun _ -> gio_pre pi) x []) ==>  
+        behavior res' `included_in id` empty_set ()))
+    | None ->  behavior res' `included_in id` empty_set ())) =
   Classical.forall_intro (_export_IOStHist_lemma (fun _ -> gio_pre pi) (fun _ -> gio_post pi) f)
 
-let export_GIO_lemma' 
+let export_GIO_lemma'
   #t1 {| d1:importable t1 |} 
   #t2 {| d2:exportable t2 |}
   (pi:check_type)
   (f:(x:t1 -> GIO t2 pi)) : 
   Lemma (forall (x':d1.itype). (
+    let ef : d1.itype -> M4 d2.etype = _export_IOStHist_arrow_spec (fun _ -> gio_pre pi) (fun _ -> gio_post pi) f in
+    let res' = reify (ef x') (fun _ -> True) in
     match import x' with
     | Some x -> (
-        let ef : d1.itype -> M4 d2.etype = _export_IOStHist_arrow_spec (fun _ -> gio_pre pi) (fun _ -> gio_post pi) f in
-        let res' = reify (ef x') (fun _ -> True) in
-
-        let f' = reify (f x) (gio_post pi []) in
-
-        check2 #t1 #events_trace #(fun _ -> gio_pre pi) x [] == true ==>  behavior res' `included_in` behavior (f' []))
-    | None -> True)) =
+      let f' = reify (f x) (gio_post pi []) in
+      (check2 #t1 #events_trace #(fun _ -> gio_pre pi) x [] ==>  
+        behavior res' `included_in (inl_app (compose export cdr))` behavior (f' [])) /\
+      (~(check2 #t1 #events_trace #(fun _ -> gio_pre pi) x []) ==>  
+        behavior res' `included_in id` empty_set ()))
+    | None ->  behavior res' `included_in id` empty_set ())) =
   Classical.forall_intro (_export_IOStHist_lemma (fun _ -> gio_pre pi) (fun _ -> gio_post pi) f)
 
-let rsp_left 
+let rsp_simple_linking
   (a : Type) {| d1:exportable a |}
   (b : Type) {| d2:ml b |}
   (c : Type) {| d3:exportable c |}
+  (pi_as_set : set_of_traces (maybe (events_trace * c)))
   (pi : check_type)
-  (p : ((ct:(a -> GIO b pi)) -> GIO c pi))
-  (ct : (d1.etype -> M4 b)) :
-  Lemma (forall (pi_as_set:set_of_traces).
+  (ps : (a -> GIO b pi) -> GIO c pi)
+  (ct : d1.etype -> M4 b) :
+  Lemma
+    (requires (forall (cs:(a -> GIO b pi)). 
+      behavior (reify (ps cs) (gio_post pi []) []) `included_in id` pi_as_set))
+    (ensures (
+      let pt : (d1.etype -> M4 b) -> M4 d3.etype = _export_IOStHist_arrow_spec (fun _ -> gio_pre pi) (fun _ -> gio_post pi) ps in
+      behavior (reify (pt ct) (fun _ -> True)) `included_in (inl_app (compose export cdr))` pi_as_set)) = 
     match import ct with
-    | Some (ct' : (pi:check_type) -> a -> GIO b pi) -> 
-        let pct : unit -> GIO c pi = fun _ -> p (ct' pi) in
-        let pct' : unit -> M4 d3.etype = _export_IOStHist_arrow_spec (fun _ -> gio_pre pi) (fun _ -> gio_post pi) pct in
-        behavior (reify (pct ()) (gio_post pi []) []) `included_in` pi_as_set ==> 
-        behavior (reify (pct' ()) (fun _ -> True)) `included_in` pi_as_set
-    | None -> False) // by (explode (); bump_nth 10; explode (); dump "h")
-  = 
-  match import ct with
-  | Some (ct' : (pi:check_type) -> a -> GIO b pi) -> 
-      let pct : unit -> GIO c pi = fun _ -> p (ct' pi) in
-      export_GIO_lemma pi pct;
-      let pct' : unit -> M4 d3.etype = _export_IOStHist_arrow_spec (fun _ -> gio_pre pi) (fun _ -> gio_post pi) pct in
-      export_GIO_lemma' pi pct;
-      calc (included_in) {
-        behavior (reify (pct' ()) (fun _ -> True));
-        `included_in` { _ by (dump "h") }
-        behavior (reify (pct ()) (gio_post pi []) []);
-        `included_in` {}
-        behavior (reify (p (ct' pi)) (gio_post pi []) []);
-      }
-  | None -> ()
+    | Some (cs : a -> GIO b pi) -> 
+      assert (behavior (reify (ps cs) (gio_post pi []) []) `included_in id` pi_as_set) by (
+        let prepost = match (List.Tot.nth (cur_binders ()) 11) with
+          | Some y -> y | None -> fail "no wp?" in
+        let (pre, post) = destruct_and (binder_to_term prepost) in
+        let pre = instantiate pre (fresh_uvar None) in
+        apply pre);
+      
+        let pt : (d1.etype -> M4 b) -> M4 d3.etype = _export_IOStHist_arrow_spec (fun _ -> gio_pre pi) (fun _ -> gio_post pi) ps in
+        let ws : unit -> GIO c pi = fun _ -> ps cs in
+        assert (behavior (reify (ws ()) (gio_post pi []) []) `included_in id` 
+          behavior (reify (ps cs) (gio_post pi []) []));
+        let wt : unit -> M4 d3.etype = _export_IOStHist_arrow_spec (fun _ -> gio_pre pi) (fun _ -> gio_post pi) ws in
+        let included_in_id #a = included_in #a #a (id #a) in
+        calc (included_in_id) {
+          behavior (reify (pt ct) (fun _ -> True));
+          // TODO: Cezar: I try to show that ((export ps) ct) == (export (ps (import ct))).
+          // I am not sure how to rewrite and unfold things.
+          `included_in_id` { admit () }
+          behavior (reify (wt ()) (fun _ -> True));
+        };
+        export_GIO_lemma' pi ws;
+        // TODO: Cezar: I should get this from the previous lemma. I am not sure why is not 
+        // accepted.
+        assume (check2 #unit #events_trace #(fun _ -> gio_pre pi) () [] ==>  behavior (reify (wt ()) (fun _ -> True)) `included_in (inl_app (compose export cdr))` behavior (reify (ws ()) (gio_post pi []) []));
+        ()
+    | None -> ()
